...

HouLean/Meta/SpecializeAndSimp2/Encoding/Option.lean
@@ -2,68 +2,25 @@ import HouLean.Meta.SpecializeAndSimp2.Encoding
 
 open Lean
 
-namespace HouLean.Meta.Sas
+-- namespace HouLean.Meta.Sas
 
-namespace OptionEncoding
+/-! ## Option Encoding -/
+def Option.decode (x : α) (valid : Bool) : Option α :=
+  if valid then some x else none
 
--- open Lean Elab Term Command Qq
--- elab "type_encoding " bs:bracketedBinder* " : " r:term ":=" b:term : command => do
---   runTermElabM fun ctx => do
---   elabBinders bs fun xs => do
---     let ret ← elabTermAndSynthesize r none
---     let decls ← (ctx ++ xs).mapM (fun x => do pure (← x.fvarId!.getUserName, (Expr.const ``Expr [])))
+namespace Option
 
---     Meta.withLocalDeclsDND decls fun xs' => do
---       let returnType := q(MetaM Unit)
---       let body ← elabTermAndSynthesize b returnType
---   pure ()
+@[simp] theorem decode_true (x : α) : Option.decode x true = some x := by simp [Option.decode]
+@[simp] theorem decode_false (x : α) : Option.decode x false = none := by simp [Option.decode]
 
--- variable (a b : Nat)
+@[simp] theorem decode_getD (x y : α) (valid : Bool) :
+    (Option.decode x valid).getD y = if valid then x else y := by
+  cases valid <;> simp [Option.decode]
 
+@[simp] theorem decode_isSome (x : α) (valid : Bool) :
+    (Option.decode x valid).isSome = valid := by
+  cases valid <;> simp [Option.decode]
 
--- open Lean Meta
-
--- type_encoding {F F' Xs Y} [Uncurry F Xs Y] [TypeEncoding F (Y:=Y)] [Uncurry F' (Bool × Xs) (Option Y)] :
---     TypeEncoding F' (Xs:=Bool×Xs) (Y:=Option Y) := do
-
---   let decoderType ← mkAppM ``TypeEncoding.Decoder #[enc]
-
-
---   forallTelescope decoderType fun xs r => do
---   withLocalDeclD `valid q(Bool) fun valid => do
---     let newDecoderType ← mkForallFVars (#[valid] ++ xs) (← mkAppM ``Option #[r])
---     -- let
---     let a := α
---     pure ()
-
-instance {α : Type u} [Inhabited α] :
-    TypeEncoding (α → Bool → Option α) where
-  encode x := (x.getD default, x.isSome)
-  decode x valid := if valid then some x else none
-  valid := by funext x; cases x <;> simp[uncurry]
-
-
-end OptionEncoding
-
-
-
-
-structure TypeEncoding' (Y : Type) (X : Fin n → Type) where
-  encode : Y → (i : Fin n) → X i
-  decode : ((i : Fin n) → X i) → Y
-  valid : decode ∘ encode = id
-
-
-
--- structure TypeEncoding (Y : Type) where
---   Decoder : Type
---   {Xs : Type}
---   [unc : Uncurry Decoder Xs Y]
---   encode : Y → Xs
---   decode : Decoder
---   valid : ∀ y, (uncurry decode) (encode y) = y
-
--- def asdf : TypeEncoding (Option Nat) := {
---   Decoder := Nat → Bool → Option Nat
---   decode := sorry
---   valid := sorry
+@[simp] theorem decode_isNone (x : α) (valid : Bool) :
+    (Option.decode x valid).isNone = !valid := by
+  cases valid <;> simp [Option.decode]
